NuStd_Base.thy
@@ -1,7 +1,7 @@
 theory NuStd_Base
   imports NuSys NuBasicAbstractors NuInstructions
   keywords
-     "\<up>:" "\<Up>:" "\<down>:" "\<Down>:" "subj" "always" "heap" "--" :: quasi_command
+     "\<up>:" "\<Up>:" "\<down>:" "\<Down>:" "subj" "always" "--" :: quasi_command
   abbrevs "|^" = "\<up>"
     and "||^" = "\<Up>"
     and "|v" = "\<down>"
@@ -313,8 +313,12 @@ theorem drop_\<nu>app: "\<^bold>p\<^bold>r\<^bold>o\<^bold>c op_drop \<blangle> 
 subsubsection \<open>duplication\<close>
 
 declare op_dup_def[\<nu>instr]
-theorem dup_\<nu>app: "\<^bold>p\<^bold>r\<^bold>o\<^bold>c op_dup \<blangle> R\<heavy_comma> X\<heavy_comma> \<^bold>h\<^bold>e\<^bold>a\<^bold>p Nothing \<longmapsto> R\<heavy_comma> X\<heavy_comma> X\<heavy_comma> \<^bold>h\<^bold>e\<^bold>a\<^bold>p Nothing\<brangle>"
-  unfolding \<nu>def op_dup_def by (auto simp add: nu_exps)
+lemma bring:
+  "\<^bold>i\<^bold>n\<^bold>d\<^bold>e\<^bold>x idx \<blangle> X \<^bold>@ R \<brangle> \<Longrightarrow> \<^bold>p\<^bold>r\<^bold>o\<^bold>c op_dup idx \<blangle> R\<heavy_comma> \<^bold>h\<^bold>e\<^bold>a\<^bold>p Nothing \<longmapsto> R\<heavy_comma> X\<heavy_comma> \<^bold>h\<^bold>e\<^bold>a\<^bold>p Nothing\<brangle>"
+  unfolding \<nu>def op_dup_def \<nu>index_def by (auto simp add: nu_exps)
+
+lemmas "&_\<nu>app" = bring
+lemmas dup_\<nu>app = bring[OF index_left_getter, OF index_here_getter]
 
 
 subsubsection \<open>pair & de-pair\<close>
@@ -493,7 +497,7 @@ proc while: \<open>S'\<heavy_comma> \<^bold>h\<^bold>e\<^bold>a\<^bold>p H'\<clo
   requires [unfolded Variant_Cast_def, simp]: "Variant_Cast vars S' H' S H"
     and Cond_\<nu>app: "\<forall>x. \<^bold>p\<^bold>r\<^bold>o\<^bold>c Cond \<blangle> S x\<heavy_comma> \<^bold>h\<^bold>e\<^bold>a\<^bold>p H x \<longmapsto> \<exists>* x'. (S x'\<heavy_comma> cond x' \<tycolon> \<bool>\<heavy_comma> \<^bold>h\<^bold>e\<^bold>a\<^bold>p H x')\<brangle>"
     and Body_\<nu>app: "\<forall>x. \<^bold>p\<^bold>r\<^bold>e\<^bold>m\<^bold>i\<^bold>s\<^bold>e cond x \<longrightarrow> \<^bold>p\<^bold>r\<^bold>o\<^bold>c Body \<blangle> S x\<heavy_comma> \<^bold>h\<^bold>e\<^bold>a\<^bold>p H x \<longmapsto> \<exists>* x'. (S x'\<heavy_comma> \<^bold>h\<^bold>e\<^bold>a\<^bold>p H x') \<brangle>"
-  \<bullet> Cond if \<medium_left_bracket> do_while x' \<open>cond x'\<close> \<medium_left_bracket> Body Cond \<medium_right_bracket> subj \<open>\<not> cond x'\<close> \<medium_right_bracket>
+  \<bullet> Cond if \<medium_left_bracket> do_while var x' \<open>cond x'\<close> \<medium_left_bracket> Body Cond \<medium_right_bracket> subj \<open>\<not> cond x'\<close> \<medium_right_bracket>
   \<bullet> \<medium_left_bracket> generalize \<open>x'\<close> x' \<open>\<lambda>x'. \<not> cond x'\<close> \<medium_right_bracket>
   finish
 
@@ -545,38 +549,38 @@ subsubsection \<open>Integer\<close>
 
 lemma [\<nu>intro]:
   "\<^bold>p\<^bold>r\<^bold>e\<^bold>m\<^bold>i\<^bold>s\<^bold>e (numeral x :: nat) < 2^LENGTH('w) \<Longrightarrow>
-   \<^bold>c\<^bold>o\<^bold>n\<^bold>s\<^bold>t\<^bold>r\<^bold>u\<^bold>c\<^bold>t ((numeral x) \<tycolon> \<nat>['w]) \<^bold>b\<^bold>y \<^bold>p\<^bold>r\<^bold>o\<^bold>c op_const_int TYPE('w::len) (numeral x)
+   \<^bold>m\<^bold>a\<^bold>k\<^bold>e ((numeral x) \<tycolon> \<nat>['w]) \<^bold>b\<^bold>y \<^bold>p\<^bold>r\<^bold>o\<^bold>c op_const_int TYPE('w::len) (numeral x)
     \<blangle> R\<heavy_comma> \<^bold>h\<^bold>e\<^bold>a\<^bold>p H \<longmapsto> R \<heavy_comma> (numeral x) \<tycolon> \<nat>['w]\<heavy_comma> \<^bold>h\<^bold>e\<^bold>a\<^bold>p H \<brangle>"
   unfolding op_const_int_def \<nu>def including show_more1 by (auto simp add: nu_exps) (metis mod_if unat_bintrunc unat_numeral)
   \<comment> \<open>Only literal number could be constructed automatically\<close>
 
 lemma [\<nu>intro]:
-  "\<^bold>c\<^bold>o\<^bold>n\<^bold>s\<^bold>t\<^bold>r\<^bold>u\<^bold>c\<^bold>t (0 \<tycolon> \<nat>['w]) \<^bold>b\<^bold>y \<^bold>p\<^bold>r\<^bold>o\<^bold>c op_const_int TYPE('w::len) 0
+  "\<^bold>m\<^bold>a\<^bold>k\<^bold>e (0 \<tycolon> \<nat>['w]) \<^bold>b\<^bold>y \<^bold>p\<^bold>r\<^bold>o\<^bold>c op_const_int TYPE('w::len) 0
     \<blangle> R\<heavy_comma> \<^bold>h\<^bold>e\<^bold>a\<^bold>p H \<longmapsto> R \<heavy_comma> 0 \<tycolon> \<nat>['w]\<heavy_comma> \<^bold>h\<^bold>e\<^bold>a\<^bold>p H \<brangle>"
-  unfolding AutoConstruct_def \<nu>def op_const_int_def by (auto simp add: nu_exps)
+  unfolding MakeTag_def \<nu>def op_const_int_def by (auto simp add: nu_exps)
 
 lemma [\<nu>intro]:
-  "\<^bold>c\<^bold>o\<^bold>n\<^bold>s\<^bold>t\<^bold>r\<^bold>u\<^bold>c\<^bold>t (1 \<tycolon> \<nat>['w]) \<^bold>b\<^bold>y \<^bold>p\<^bold>r\<^bold>o\<^bold>c op_const_int TYPE('w::len) 1
+  "\<^bold>m\<^bold>a\<^bold>k\<^bold>e (1 \<tycolon> \<nat>['w]) \<^bold>b\<^bold>y \<^bold>p\<^bold>r\<^bold>o\<^bold>c op_const_int TYPE('w::len) 1
     \<blangle> R\<heavy_comma> \<^bold>h\<^bold>e\<^bold>a\<^bold>p H \<longmapsto> R\<heavy_comma> 1 \<tycolon> \<nat>['w]\<heavy_comma> \<^bold>h\<^bold>e\<^bold>a\<^bold>p H \<brangle>"
-  unfolding AutoConstruct_def \<nu>def op_const_int_def by (auto simp add: nu_exps)
+  unfolding MakeTag_def \<nu>def op_const_int_def by (auto simp add: nu_exps)
 
 lemma [\<nu>intro]:
   "\<^bold>p\<^bold>r\<^bold>e\<^bold>m\<^bold>i\<^bold>s\<^bold>e (numeral x :: nat) < 2^LENGTH('w) \<Longrightarrow>
-   \<^bold>c\<^bold>o\<^bold>n\<^bold>s\<^bold>t\<^bold>r\<^bold>u\<^bold>c\<^bold>t ((numeral x) \<tycolon> \<nat>\<^sup>r['w]) \<^bold>b\<^bold>y \<^bold>p\<^bold>r\<^bold>o\<^bold>c op_const_int TYPE('w::len) (numeral x)
+   \<^bold>m\<^bold>a\<^bold>k\<^bold>e ((numeral x) \<tycolon> \<nat>\<^sup>r['w]) \<^bold>b\<^bold>y \<^bold>p\<^bold>r\<^bold>o\<^bold>c op_const_int TYPE('w::len) (numeral x)
     \<blangle> R\<heavy_comma> \<^bold>h\<^bold>e\<^bold>a\<^bold>p H \<longmapsto> R\<heavy_comma> (numeral x) \<tycolon> \<nat>\<^sup>r['w]\<heavy_comma> \<^bold>h\<^bold>e\<^bold>a\<^bold>p H \<brangle>"
   unfolding op_const_int_def \<nu>def including show_more1 by (auto simp add: nu_exps)
 
 lemma [\<nu>intro]:
-  "\<^bold>c\<^bold>o\<^bold>n\<^bold>s\<^bold>t\<^bold>r\<^bold>u\<^bold>c\<^bold>t (0 \<tycolon> \<nat>\<^sup>r['w]) \<^bold>b\<^bold>y \<^bold>p\<^bold>r\<^bold>o\<^bold>c op_const_int TYPE('w::len) 0 \<blangle> R\<heavy_comma> \<^bold>h\<^bold>e\<^bold>a\<^bold>p H \<longmapsto> R\<heavy_comma> 0 \<tycolon> \<nat>\<^sup>r['w]\<heavy_comma> \<^bold>h\<^bold>e\<^bold>a\<^bold>p H \<brangle>"
+  "\<^bold>m\<^bold>a\<^bold>k\<^bold>e (0 \<tycolon> \<nat>\<^sup>r['w]) \<^bold>b\<^bold>y \<^bold>p\<^bold>r\<^bold>o\<^bold>c op_const_int TYPE('w::len) 0 \<blangle> R\<heavy_comma> \<^bold>h\<^bold>e\<^bold>a\<^bold>p H \<longmapsto> R\<heavy_comma> 0 \<tycolon> \<nat>\<^sup>r['w]\<heavy_comma> \<^bold>h\<^bold>e\<^bold>a\<^bold>p H \<brangle>"
   unfolding op_const_int_def \<nu>def including show_more1 by (auto simp add: nu_exps)
 
 lemma [\<nu>intro]:
-  "\<^bold>c\<^bold>o\<^bold>n\<^bold>s\<^bold>t\<^bold>r\<^bold>u\<^bold>c\<^bold>t (1 \<tycolon> \<nat>\<^sup>r['w]) \<^bold>b\<^bold>y \<^bold>p\<^bold>r\<^bold>o\<^bold>c op_const_int TYPE('w::len) 1 \<blangle> R\<heavy_comma> \<^bold>h\<^bold>e\<^bold>a\<^bold>p H \<longmapsto> R\<heavy_comma> 1 \<tycolon> \<nat>\<^sup>r['w]\<heavy_comma> \<^bold>h\<^bold>e\<^bold>a\<^bold>p H \<brangle>"
+  "\<^bold>m\<^bold>a\<^bold>k\<^bold>e (1 \<tycolon> \<nat>\<^sup>r['w]) \<^bold>b\<^bold>y \<^bold>p\<^bold>r\<^bold>o\<^bold>c op_const_int TYPE('w::len) 1 \<blangle> R\<heavy_comma> \<^bold>h\<^bold>e\<^bold>a\<^bold>p H \<longmapsto> R\<heavy_comma> 1 \<tycolon> \<nat>\<^sup>r['w]\<heavy_comma> \<^bold>h\<^bold>e\<^bold>a\<^bold>p H \<brangle>"
   unfolding op_const_int_def \<nu>def including show_more1 by (auto simp add: nu_exps)
 
 
 lemma [\<nu>intro 1100]:
-  "\<^bold>c\<^bold>o\<^bold>n\<^bold>s\<^bold>t\<^bold>r\<^bold>u\<^bold>c\<^bold>t ((numeral x) \<tycolon> \<nat>[size_t]) \<^bold>b\<^bold>y \<^bold>p\<^bold>r\<^bold>o\<^bold>c op_const_size_t (numeral x)
+  "\<^bold>m\<^bold>a\<^bold>k\<^bold>e ((numeral x) \<tycolon> \<nat>[size_t]) \<^bold>b\<^bold>y \<^bold>p\<^bold>r\<^bold>o\<^bold>c op_const_size_t (numeral x)
     \<blangle> R\<heavy_comma> \<^bold>h\<^bold>e\<^bold>a\<^bold>p H \<longmapsto> R\<heavy_comma> (numeral x) \<tycolon> \<nat>[size_t]\<heavy_comma> \<^bold>h\<^bold>e\<^bold>a\<^bold>p H \<brangle>"
   unfolding op_const_size_t_def \<nu>def by (auto simp add: nu_exps nat_take_bit_eq take_bit_nat_eq_self_iff)
 
@@ -600,7 +604,7 @@ subsubsection \<open>Integer\<close>
 (* theorem const_nat_round_\<nu>app: "\<^bold>p\<^bold>r\<^bold>o\<^bold>c op_const_int TYPE('w::len) (of_nat n) \<blangle> R \<longmapsto> R \<heavy_comma> n \<tycolon> \<nat>\<^sup>r['w] \<brangle>"
   unfolding \<nu>def op_const_int_def by auto *)
 
-(* schematic_goal "\<^bold>c\<^bold>o\<^bold>n\<^bold>s\<^bold>t\<^bold>r\<^bold>u\<^bold>c\<^bold>t 3 \<^bold>b\<^bold>y \<^bold>p\<^bold>r\<^bold>o\<^bold>c ?f
+(* schematic_goal "\<^bold>m\<^bold>a\<^bold>k\<^bold>e 3 \<^bold>b\<^bold>y \<^bold>p\<^bold>r\<^bold>o\<^bold>c ?f
   \<blangle>\<flower_L>\<medium_left_bracket> A \<flower_L>\<flower>\<flower_R>X\<medium_right_bracket>\<flower_R>   \<longmapsto> ?T \<brangle>" by (rule \<nu>intro) *)
 
 (* instantiation typing :: (lrep, plus) plus begin
@@ -648,22 +652,61 @@ lemma boolean_not_\<nu>app[\<nu>overload not]:
 
 subsection \<open>Field Index\<close>
 
+lemma [\<nu>intro]:
+  "\<^bold>f\<^bold>i\<^bold>e\<^bold>l\<^bold>d \<^bold>i\<^bold>n\<^bold>d\<^bold>e\<^bold>x idx \<blangle> X \<^bold>@ A \<brangle> \<^bold>g\<^bold>e\<^bold>t g \<^bold>m\<^bold>a\<^bold>p m
+    \<Longrightarrow> \<^bold>f\<^bold>i\<^bold>e\<^bold>l\<^bold>d \<^bold>i\<^bold>n\<^bold>d\<^bold>e\<^bold>x index_tuple idx \<blangle> X \<^bold>@ \<lbrace> A \<rbrace> \<brangle> \<^bold>g\<^bold>e\<^bold>t g \<^bold>m\<^bold>a\<^bold>p m"
+  unfolding FieldIndex_def \<nu>index_def index_tuple_def
+  by (cases idx) (simp add: tuple_forall nu_exps)
+
+lemma [\<nu>intro]:
+  "\<^bold>m\<^bold>a\<^bold>k\<^bold>e Suc i \<^bold>b\<^bold>y \<^bold>i\<^bold>n\<^bold>d\<^bold>e\<^bold>x idx \<blangle> X \<^bold>@ a \<tycolon> A \<brangle> \<Longrightarrow>
+   \<^bold>m\<^bold>a\<^bold>k\<^bold>e Suc i \<^bold>b\<^bold>y \<^bold>i\<^bold>n\<^bold>d\<^bold>e\<^bold>x index_tuple idx \<blangle> X \<^bold>@ a \<tycolon> \<lbrace> A \<rbrace> \<brangle>"
+  unfolding \<nu>index_def  MakeTag_def index_tuple_def by (cases idx) (simp add: nu_exps tuple_forall)
+lemma [\<nu>intro]:
+  "\<^bold>m\<^bold>a\<^bold>k\<^bold>e Suc i \<^bold>b\<^bold>y \<^bold>i\<^bold>n\<^bold>d\<^bold>e\<^bold>x idx \<blangle> X \<^bold>@ a \<tycolon> A \<longmapsto> Y \<^bold>@ b \<tycolon> B \<brangle> \<Longrightarrow>
+   \<^bold>m\<^bold>a\<^bold>k\<^bold>e Suc i \<^bold>b\<^bold>y \<^bold>i\<^bold>n\<^bold>d\<^bold>e\<^bold>x index_tuple idx \<blangle> X \<^bold>@ a \<tycolon> \<lbrace> A \<rbrace> \<longmapsto> Y \<^bold>@ b \<tycolon> \<lbrace> B \<rbrace> \<brangle>"
+  unfolding \<nu>index_def  MakeTag_def index_tuple_def by (cases idx) (simp add: nu_exps tuple_forall)
+lemma [\<nu>intro]:
+  "\<^bold>m\<^bold>a\<^bold>k\<^bold>e Suc i \<^bold>b\<^bold>y \<^bold>f\<^bold>i\<^bold>e\<^bold>l\<^bold>d \<^bold>i\<^bold>n\<^bold>d\<^bold>e\<^bold>x idx \<blangle> X \<^bold>@ A \<brangle> \<^bold>g\<^bold>e\<^bold>t g \<^bold>m\<^bold>a\<^bold>p m
+    \<Longrightarrow> \<^bold>m\<^bold>a\<^bold>k\<^bold>e Suc i \<^bold>b\<^bold>y \<^bold>f\<^bold>i\<^bold>e\<^bold>l\<^bold>d \<^bold>i\<^bold>n\<^bold>d\<^bold>e\<^bold>x index_tuple idx \<blangle> X \<^bold>@ \<lbrace> A \<rbrace> \<brangle> \<^bold>g\<^bold>e\<^bold>t g \<^bold>m\<^bold>a\<^bold>p m"
+  unfolding FieldIndex_def \<nu>index_def index_tuple_def
+  by (cases idx) (simp add: tuple_forall nu_exps)
+
+lemma [\<nu>intro]:
+  "\<^bold>m\<^bold>a\<^bold>k\<^bold>e i#l \<^bold>b\<^bold>y \<^bold>i\<^bold>n\<^bold>d\<^bold>e\<^bold>x idx \<blangle> X \<^bold>@ a \<tycolon> A \<brangle> \<Longrightarrow>
+   \<^bold>m\<^bold>a\<^bold>k\<^bold>e i#l \<^bold>b\<^bold>y \<^bold>i\<^bold>n\<^bold>d\<^bold>e\<^bold>x index_tuple idx \<blangle> X \<^bold>@ a \<tycolon> \<lbrace> A \<rbrace> \<brangle>"
+  unfolding \<nu>index_def  MakeTag_def index_tuple_def by (cases idx) (simp add: nu_exps tuple_forall)
+lemma [\<nu>intro]:
+  "\<^bold>m\<^bold>a\<^bold>k\<^bold>e i#l \<^bold>b\<^bold>y \<^bold>i\<^bold>n\<^bold>d\<^bold>e\<^bold>x idx \<blangle> X \<^bold>@ a \<tycolon> A \<longmapsto> Y \<^bold>@ b \<tycolon> B \<brangle> \<Longrightarrow>
+   \<^bold>m\<^bold>a\<^bold>k\<^bold>e i#l \<^bold>b\<^bold>y \<^bold>i\<^bold>n\<^bold>d\<^bold>e\<^bold>x index_tuple idx \<blangle> X \<^bold>@ a \<tycolon> \<lbrace> A \<rbrace> \<longmapsto> Y \<^bold>@ b \<tycolon> \<lbrace> B \<rbrace> \<brangle>"
+  unfolding \<nu>index_def  MakeTag_def index_tuple_def by (cases idx) (simp add: nu_exps tuple_forall)
+lemma [\<nu>intro]:
+  "\<^bold>m\<^bold>a\<^bold>k\<^bold>e i#l \<^bold>b\<^bold>y \<^bold>f\<^bold>i\<^bold>e\<^bold>l\<^bold>d \<^bold>i\<^bold>n\<^bold>d\<^bold>e\<^bold>x idx \<blangle> X \<^bold>@ A \<brangle> \<^bold>g\<^bold>e\<^bold>t g \<^bold>m\<^bold>a\<^bold>p m
+    \<Longrightarrow> \<^bold>m\<^bold>a\<^bold>k\<^bold>e i#l \<^bold>b\<^bold>y \<^bold>f\<^bold>i\<^bold>e\<^bold>l\<^bold>d \<^bold>i\<^bold>n\<^bold>d\<^bold>e\<^bold>x index_tuple idx \<blangle> X \<^bold>@ \<lbrace> A \<rbrace> \<brangle> \<^bold>g\<^bold>e\<^bold>t g \<^bold>m\<^bold>a\<^bold>p m"
+  unfolding FieldIndex_def \<nu>index_def index_tuple_def
+  by (cases idx) (simp add: tuple_forall nu_exps)
+
 subsubsection \<open>Abstraction\<close>
 
-definition FieldIndex :: " ('a,'a,'ax,'ax) index \<Rightarrow> ('ax::lrep,'bx) \<nu> \<Rightarrow> ('a::lrep,'b) \<nu> \<Rightarrow> ('b \<Rightarrow> 'bx) \<Rightarrow> (('bx \<Rightarrow> 'bx) \<Rightarrow> 'b \<Rightarrow> 'b) \<Rightarrow>bool"
-  where "FieldIndex adr X A gt mp \<longleftrightarrow> (\<forall>a f. \<^bold>i\<^bold>n\<^bold>d\<^bold>e\<^bold>x adr \<blangle> \<tort_lbrace>gt a \<tycolon> X\<tort_rbrace> \<^bold>@ \<tort_lbrace>a \<tycolon> A\<tort_rbrace> \<longmapsto> \<tort_lbrace>f (gt a) \<tycolon> X\<tort_rbrace> \<^bold>@ \<tort_lbrace>mp f a \<tycolon> A\<tort_rbrace> \<brangle>)"
 
-lemma FieldIndex_here: "FieldIndex index_here X X id id"
-  unfolding FieldIndex_def \<nu>index_def index_here_def by auto
-lemma FieldIndex_left: "FieldIndex f X A gt mp \<Longrightarrow> FieldIndex (index_left f) X (A \<cross_product> R) (gt o fst) (apfst o mp)"
-  unfolding FieldIndex_def \<nu>index_def index_left_def by (auto simp add: nu_exps)
-lemma FieldIndex_right: "FieldIndex f X A gt mp \<Longrightarrow> FieldIndex (index_right f) X (R \<cross_product> A) (gt o snd) (apsnd o mp)"
-  unfolding FieldIndex_def \<nu>index_def index_right_def by (auto simp add: nu_exps)
+\<nu>processor field_index 110 \<open>\<^bold>i\<^bold>n\<^bold>d\<^bold>e\<^bold>x adr \<blangle> X \<^bold>@ A \<brangle> \<Longrightarrow> PROP P\<close> \<open>fn ctx => fn sequent =>
+  Parse.nat >> (fn i => fn _ =>
+  let open NuBasics NuHelp
+    val A = Thm.major_prem_of sequent |> dest_Trueprop |> dest_triop \<^const_name>\<open>AdrGet\<close> |> #3
+    val A = repeat (dest_monop \<^const_name>\<open>NuTuple\<close>)
+    val arity = 1
+val _ =
+Logic.dest_implies (prop_of sequent) |> #1
+        |> dest_Trueprop |> dest_quinop \<^const_name>\<open>FieldIndex\<close> |> #3
+        |> dest_monop \<^const_name>\<open>NuTuple\<close> |> strip_binop_r \<^const_name>\<open>Fusion\<close> |> length
+    val path1 = funpow (i-1) (fn th => th RS @{thm FieldIndex_right})
+        (@{thm FieldIndex_here}
+              |> (fn th => if arity = i then th else th RS @{thm FieldIndex_left}))
+  in 
+    (path1 RS (@{thm FieldIndex_tupl} RS major), ctx)
+  end)\<close>
 
-lemma FieldIndex_tupl: "FieldIndex f X A gt mp \<Longrightarrow> FieldIndex (index_enter_tup f) X \<lbrace> A \<rbrace> gt mp"
-  unfolding FieldIndex_def \<nu>index_def index_enter_tup_def by (auto simp add: tuple_forall nu_exps)
-
-\<nu>processor field_index 110 \<open>FieldIndex f X \<lbrace> A \<rbrace> gt mp \<Longrightarrow> PROP P\<close> \<open>fn ctx => fn major => Parse.nat >> (fn i => fn _ =>
+\<nu>processor field_index_getter 110 \<open>FieldIndex f X \<lbrace> A \<rbrace> gt mp \<Longrightarrow> PROP P\<close> \<open>fn ctx => fn major => Parse.nat >> (fn i => fn _ =>
   let open NuBasics NuHelp
     val arity = Logic.dest_implies (prop_of major) |> #1
         |> dest_Trueprop |> dest_quinop \<^const_name>\<open>FieldIndex\<close> |> #3
@@ -789,14 +832,14 @@ subsubsection \<open>Load & Store\<close>
 abbreviation "list_map_at f i l \<equiv> list_update l i (f (l ! i))"
 
 lemma op_load[ \<nu>overload "\<up>:" ]:
-  "FieldIndex field_index Y X gt mp \<longrightarrow>
+  "\<^bold>(\<^bold>( \<^bold>i\<^bold>n\<^bold>d\<^bold>e\<^bold>x field_index \<blangle> y \<tycolon> Y \<^bold>@ x \<tycolon> X \<brangle> \<^bold>)\<^bold>) \<longrightarrow>
   \<^bold>p\<^bold>r\<^bold>o\<^bold>c op_load TYPE('y::field) TYPE('x) field_index
-    \<blangle> R\<heavy_comma> addr \<tycolon> Pointer\<heavy_comma> \<^bold>h\<^bold>e\<^bold>a\<^bold>p H \<heavy_asterisk> addr \<R_arr_tail> x \<tycolon> Ref X \<longmapsto> R\<heavy_comma> gt x \<tycolon> Y\<heavy_comma> \<^bold>h\<^bold>e\<^bold>a\<^bold>p H \<heavy_asterisk> addr \<R_arr_tail> x \<tycolon> Ref X\<brangle> "
+    \<blangle> R\<heavy_comma> addr \<tycolon> Pointer\<heavy_comma> \<^bold>h\<^bold>e\<^bold>a\<^bold>p H \<heavy_asterisk> addr \<R_arr_tail> x \<tycolon> Ref X \<longmapsto> R\<heavy_comma> y \<tycolon> Y\<heavy_comma> \<^bold>h\<^bold>e\<^bold>a\<^bold>p H \<heavy_asterisk> addr \<R_arr_tail> x \<tycolon> Ref X\<brangle> "
   for X :: "('x::field, 'c) \<nu>"
-  unfolding op_load_def Procedure_def FieldIndex_def \<nu>index_def Heap_Divider_def
+  unfolding op_load_def Procedure_def \<nu>index_def Heap_Divider_def Protector_def
   by (cases field_index, cases addr)  (auto simp add: lrep_exps MemAddrState_def nu_exps split: option.split iff: addr_allocated_def)
 
-lemmas [ \<nu>overload "\<up>" ] = op_load[THEN mp, OF FieldIndex_here, simplified]
+lemmas [ \<nu>overload "\<up>" ] = op_load[THEN mp, OF Protector_I, OF index_here_getter, simplified]
 
 proc i_load_n[\<nu>overload "\<up>:"]:
   \<open>a \<tycolon> Pointer\<heavy_comma> i \<tycolon> \<nat>[size_t]\<heavy_comma> \<^bold>h\<^bold>e\<^bold>a\<^bold>p H \<heavy_asterisk> a \<R_arr_tail> xs \<tycolon> Array X\<close> \<longmapsto> \<open>gt (xs ! i) \<tycolon> Y\<heavy_comma> \<^bold>h\<^bold>e\<^bold>a\<^bold>p H \<heavy_asterisk> a \<R_arr_tail> xs \<tycolon> Array X\<close>
@@ -853,7 +896,7 @@ proc times: \<open>R'\<heavy_comma> n \<tycolon> \<nat>['b::len]\<heavy_comma> \
   requires Body: \<open>\<forall>x i. \<^bold>p\<^bold>r\<^bold>e\<^bold>m\<^bold>i\<^bold>s\<^bold>e i < n \<longrightarrow> \<^bold>p\<^bold>r\<^bold>e\<^bold>m\<^bold>i\<^bold>s\<^bold>e P x i \<longrightarrow>
       \<^bold>p\<^bold>r\<^bold>o\<^bold>c body \<blangle> R x\<heavy_comma> i \<tycolon> \<nat>['b]\<heavy_comma> \<^bold>h\<^bold>e\<^bold>a\<^bold>p H x \<longmapsto> \<exists>*x'. ((R x'\<heavy_comma> \<^bold>h\<^bold>e\<^bold>a\<^bold>p H x') \<and>\<^sup>s P x' (Suc i))\<brangle>\<close>
   \<bullet> \<rightarrow> n \<open>0 \<tycolon> \<nat>['b]\<close>
-  \<bullet> while var vars i in \<open>R vars\<close>, i heap \<open>H vars\<close> always \<open>i \<le> n \<and> P vars i\<close>
+  \<bullet> while var vars i stack \<open>R vars\<close>, i heap \<open>H vars\<close> always \<open>i \<le> n \<and> P vars i\<close>
   \<bullet> \<medium_left_bracket> dup n < \<medium_right_bracket> \<medium_left_bracket> -- i Body i 1 + cast ie \<open>Suc i\<close> \<medium_right_bracket> drop
   finish
 
